src/Typing.v
@@ -1,4 +1,4 @@
-From TLC Require Import LibString LibLN LibEnv.
+From TLC Require Import LibString LibLN.
 From MCore Require Import Syntax Tactics.
 
 Module Typing (P : PAT).
@@ -41,6 +41,7 @@ Module Typing (P : PAT).
     Reserved Notation "Gamma |= T ~:: k " (at level 50).
     Inductive ok_type : env -> type -> kind -> Prop :=
     | KVar : forall Gamma tv k,
+        ok_env Gamma ->
         binds tv (BindTVar k) Gamma ->
         Gamma |= TyFVar tv ~:: k
     | KArr : forall Gamma ty1 ty2,
@@ -73,11 +74,8 @@ Module Typing (P : PAT).
     (*     (forall {T : tname}, d2[T] \c d1[T]) -> *)
     (*     ok_type Gamma ty (KiData d2) *)
     where " Gamma |= T ~:: k " := (ok_type Gamma T k)
-    .
-    #[export]
-     Hint Constructors ok_type : mcore.
 
-    Inductive ok_env : env -> Prop :=
+    with ok_env : env -> Prop :=
     | EnvEmpty : ok_env empty
     | EnvTName : forall Gamma X, ok_env Gamma -> X # Gamma -> ok_env (Gamma & X ~ BindTName)
     | EnvCon   :
@@ -103,6 +101,8 @@ Module Typing (P : PAT).
         M # Gamma ->
         ok_env (Gamma & M ~ BindMatch m)
     .
+    #[export]
+     Hint Constructors ok_type : mcore.
     #[export]
      Hint Constructors ok_env : mcore.
 
@@ -210,17 +210,13 @@ Module Typing (P : PAT).
     (** PROPERTIES OF TYPING **)
     (**************************)
 
-    Lemma ok_type_lct :
-      forall Gamma T k,
-        Gamma |= T ~:: k ->
-        lct T.
-    Proof. introv Hk ; induction* Hk. Qed.
-
     Lemma ok_env_ok :
       forall Gamma,
         ok_env Gamma ->
         ok Gamma.
-    Proof. introv Hwf ; induction* Hwf. Qed.
+    Proof. introv Henv ; induction* Henv. Qed.
+    #[export]
+     Hint Resolve ok_env_ok : mcore.
 
     Lemma ok_kind_weakening :
       forall G3 G1 G2 k,
@@ -230,18 +226,17 @@ Module Typing (P : PAT).
 
     Lemma ok_type_weakening :
       forall G3 G1 G2 T k,
-        ok_type (G1 & G3) T k ->
+        G1 & G3 |= T ~:: k ->
         ok_env (G1 & G2 & G3) ->
-        ok_type (G1 & G2 & G3) T k.
+        G1 & G2 & G3 |= T ~:: k.
     Proof.
       introv Hk Henv.
       remember (G1 & G3) as Gamma. gen G3.
       induction* Hk; intros; substs.
-      - constructors*. apply* binds_weaken.
-        apply* ok_env_ok.
-      - apply_fresh* KAll. apply* ok_kind_weakening.
+      { Case "TyFVar". constructors*. apply* binds_weaken. }
+      { Case "TyAll". apply_fresh* KAll. apply* ok_kind_weakening.
         apply_ih_bind* H1.
-        constructor*. apply* ok_kind_weakening.
+        constructor*. apply* ok_kind_weakening. }
     Qed.
 
     Lemma ok_env_ok_type :
@@ -252,10 +247,393 @@ Module Typing (P : PAT).
     Proof.
       introv Henv Hbind.
       induction* Henv ; try (binds_cases Hbind ; apply_empty* ok_type_weakening).
-      - false. apply* binds_empty_inv.
-      - inverts* EQ.
+      { Case "EnvEmpty". false. apply* binds_empty_inv. }
+      { Case "EnvVar". inverts* EQ. }
     Qed.
 
+    Lemma ok_type_lct :
+      forall Gamma T k,
+        Gamma |= T ~:: k ->
+        lct T.
+    Proof. introv Hk ; induction* Hk. Qed.
+    #[export]
+     Hint Resolve ok_type_lct : mcore.
+
+    Lemma ok_term_lct :
+      forall Gamma t T,
+        Gamma |= t ~: T ->
+        lct T.
+    Proof with eauto using ok_env_ok_type, ok_type_lct.
+      introv hasType.
+      induction* hasType...
+      { Case "TmLam". constructors...
+        pick_fresh_gen L y... }
+      { Case "TmApp". inverts* IHhasType1. }
+      { Case "TmTyLam". inverts* IHhasType.
+        assert(Hlct: lct ty2)...
+        pick_fresh X. rewrite *(@tsubst_intro X).
+        apply* tsubst_lct. }
+    Qed.
+    #[export]
+     Hint Resolve ok_term_lct : mcore.
+
+    Lemma ok_term_lc :
+      forall Gamma t T,
+        Gamma |= t ~: T ->
+        lc t.
+    Proof with eauto using ok_term_lct, ok_type_lct with mcore.
+      introv Htype.
+      induction* Htype; intros.
+    Qed.
+    #[export]
+     Hint Resolve ok_term_lc : mcore.
+
+    Lemma ok_env_push :
+      forall G1 x b,
+        ok_env (G1 & x ~ b) ->
+        ok_env G1.
+    Proof.
+      introv Hwf.
+      inverts Hwf ; try (apply eq_push_inv in H; inverts H as []; substs*).
+      false. apply *empty_push_inv.
+    Qed.
+
+    Lemma ok_type_ok_env :
+      forall Gamma T k,
+        Gamma |= T ~:: k ->
+        ok_env Gamma.
+    Proof.
+      introv hasType.
+      induction* hasType; pick_fresh_gen L x;
+        eauto using ok_env_push.
+    Qed.
+    #[export]
+     Hint Resolve ok_type_ok_env : mcore.
+
+    Lemma ok_term_ok_env :
+      forall Gamma t T,
+        Gamma |= t ~: T ->
+        ok_env Gamma.
+    Proof.
+      introv hasType.
+      induction* hasType; pick_fresh_gen L x;
+        eauto using ok_env_push.
+    Qed.
+    #[export]
+     Hint Resolve ok_term_ok_env : mcore.
+
+    Lemma ok_term_weakening :
+      forall G3 G2 G1 t T,
+        G1 & G3 |= t ~: T ->
+        ok_env (G1 & G2 & G3) ->
+        G1 & G2 & G3 |= t ~: T.
+    Proof.
+      introv hasType Henv. remember (G1 & G3) as H. gen G3.
+      induction hasType; intros; substs*.
+      { Case "TmFVar". constructors*. apply* binds_weaken. }
+      { Case "TmLam". apply_fresh* TLam as y.
+        - apply* ok_type_weakening.
+        - apply_ih_bind* H1.
+          constructors*.
+          apply* ok_type_weakening. }
+      { Case "TmTyLam". apply_fresh* TTyLam as X.
+        - apply* ok_kind_weakening.
+        - apply_ih_bind* H1. constructors*. apply* ok_kind_weakening. }
+      { Case "TmTyApp". constructors*. apply* ok_type_weakening. }
+    Qed.
+
+    Lemma ok_data_strengthening :
+      forall G1 G2 x T d,
+        ok_data (G1 & x ~ BindVar T & G2) d ->
+        ok_data (G1 & G2) d.
+    Proof.
+      introv Hd. unfolds ok_data.
+      splits*. introv Hbind.
+      lets [Hbind' Hk]: (proj2 Hd) Hbind.
+      splits.
+      - binds_cases Hbind' ; auto.
+      - introv Hkin. lets [ ? (? & Hbindk) ] : Hk Hkin.
+        binds_cases Hbindk ; eauto.
+    Qed.
+
+    Lemma ok_kind_strengthening :
+      forall G1 G2 x T k,
+        ok_kind (G1 & x ~ BindVar T & G2) k ->
+        ok_kind (G1 & G2) k.
+    Proof. introv Hk. induction* Hk. Qed.
+
+    Lemma ok_type_strengthening :
+      forall G1 G2 x T1 T2 k,
+        G1 & x ~ BindVar T2 & G2 |= T1 ~:: k ->
+        ok_env (G1 & G2) ->
+        G1 & G2 |= T1 ~:: k.
+    Proof.
+      introv Htk. remember (G1 & x ~ BindVar T2 & G2) as G. gen G2.
+      induction Htk; intros; substs*.
+      { Case "TyFVar". constructors*.
+        binds_cases H0 ; auto. }
+      { Case "TyAll". apply_fresh* KAll as X.
+        apply* ok_kind_strengthening.
+        apply_ih_bind* H1. constructor*. apply* ok_kind_strengthening. }
+    Qed.
+
+    Lemma ok_env_con_inv :
+      forall Gamma K d ty T,
+        ok_env (Gamma & K ~ BindCon d ty T) ->
+        ok_data Gamma d /\ Gamma |= ty ~:: KiType /\ binds T BindTName Gamma.
+    Proof.
+      introv Henv.
+      inverts Henv ; try (apply eq_push_inv in H as (? & ? & ?); substs* ; splits* ; fequals).
+      false. apply* empty_push_inv.
+    Qed.
+
+    Lemma ok_env_tvar_inv :
+      forall Gamma X k,
+        ok_env (Gamma & X ~ BindTVar k) ->
+        ok_kind Gamma k.
+    Proof.
+      introv Henv.
+      inverts Henv ; try (apply eq_push_inv in H as (? & ? & ?); substs* ; fequals).
+      false. apply* empty_push_inv.
+    Qed.
+
+    Lemma ok_env_var_inv :
+      forall Gamma x T,
+        ok_env (Gamma & x ~ BindVar T) ->
+        Gamma |= T ~:: KiType.
+    Proof.
+      introv Henv.
+      inverts Henv ; try (apply eq_push_inv in H as (? & ? & ?); substs* ; fequals).
+      false. apply* empty_push_inv.
+    Qed.
+
+    Lemma ok_env_strengthening :
+      forall G1 x T G3,
+        ok_env (G1 & x ~ BindVar T & G3) ->
+        ok_env (G1 & G3).
+    Proof.
+      introv Henv. induction G3 using env_ind.
+      { Case "Empty". rewrite concat_empty_r in *. apply* ok_env_push. }
+      { Case "Push". rewrite concat_assoc in *.
+        specializes IHG3 (ok_env_push _ _ _ Henv).
+        lets [? Hdisj] : ok_push_inv (ok_env_ok _ Henv).
+        destruct v.
+        { SCase "BindTName". constructor~. }
+        { SCase "BindCon". forwards [ Hd (Htk & HT)]: ok_env_con_inv Henv.
+          constructor~.
+          - applys ok_data_strengthening Hd.
+          - applys* ok_type_strengthening Htk.
+          - binds_cases HT ; auto. }
+        { SCase "BindTVar". forwards Hk: ok_env_tvar_inv Henv.
+          constructor~. applys ok_kind_strengthening Hk. }
+        { SCase "BindVar". forwards Htk: ok_env_var_inv Henv.
+          constructor~. applys* ok_type_strengthening Htk. }
+        { SCase "BindMatch". constructor~. } }
+    Qed.
+
+    Lemma ok_term_subst :
+      forall G2 G1 x T1 T2 t1 t2,
+        G1 & x ~ BindVar T2 & G2 |= t1 ~: T1 ->
+        G1 |= t2 ~: T2 ->
+        G1 & G2 |= [x => t2]t1 ~: T1.
+    Proof with eauto using ok_term_lc, ok_env_strengthening, ok_type_strengthening with mcore.
+      introv hasType1 hasType2.
+      remember (G1 & x ~ BindVar T2 & G2) as G. gen G2.
+      induction hasType1; intros; simpls; substs...
+      { Case "TmFVar". solve_var.
+        - binds_get H0... apply_empty ok_term_weakening...
+        - binds_cases H0... }
+      { Case "TmLam". apply_fresh* TLam as y...
+        rewrite subst_open_comm... apply_ih_bind* H1. }
+      { Case "TmTyLam". apply_fresh* TTyLam as X. apply* ok_kind_strengthening.
+        rewrite* topen_t_subst_comm. apply_ih_bind* H1. }
+      { Case "TmTyApp". constructors*. apply* ok_type_strengthening. }
+    Qed.
+
+    Lemma ok_data_tvar_strengthening :
+      forall G1 G2 x k d,
+        ok_data (G1 & x ~ BindTVar k & G2) d ->
+        ok_data (G1 & G2) d.
+    Proof.
+      introv Hd. unfolds ok_data.
+      splits*. introv Hbind.
+      lets [Hbind' Hk]: (proj2 Hd) Hbind.
+      splits.
+      - binds_cases Hbind' ; auto.
+      - introv Hkin. lets [ ? (? & Hbindk) ] : Hk Hkin.
+        binds_cases Hbindk ; eauto.
+    Qed.
+
+    Lemma ok_data_bsubst :
+      forall G1 G2 X T d,
+        ok_data (G1 & G2) d ->
+        ok_data (G1 & map (bsubst X T) G2) d.
+    Proof.
+      introv Hd. unfolds ok_data.
+      splits*. introv Hbind.
+      lets [Hbind' Hk]: (proj2 Hd) Hbind.
+      splits.
+      - binds_cases Hbind' ; auto.
+        replaces BindTName with (bsubst X T BindTName) ; auto.
+      - introv Hkin. lets [ d' (ty & Hbindk) ] : Hk Hkin.
+        binds_cases Hbindk ; eauto.
+        exists d' ({X => T} ty).
+        replaces (BindCon d' ({X => T} ty) T0) with (bsubst X T (BindCon d' ty T0)) ; auto.
+    Qed.
+
+    Lemma ok_kind_tvar_strengthening :
+      forall G1 G2 x k' k,
+        ok_kind (G1 & x ~ BindTVar k' & G2) k ->
+        ok_kind (G1 & G2) k.
+    Proof. introv Hk. induction* Hk. Qed.
+
+    Lemma ok_kind_bsubst :
+      forall G1 G2 X T k,
+        ok_kind (G1 & G2) k ->
+        ok_kind (G1 & map (bsubst X T) G2) k.
+    Proof. introv Hk. induction* Hk. Qed.
+
+    Lemma ok_type_tsubst :
+      forall G1 G2 X T1 T2 k k',
+        G1 & X ~ BindTVar k' & G2 |= T1 ~:: k ->
+        G1 |= T2 ~:: k' ->
+        ok_env (G1 & map (bsubst X T2) G2) ->
+        G1 & map (bsubst X T2) G2 |= {X => T2} T1 ~:: k.
+    Proof with eauto with mcore.
+      introv Hkt1 Hkt2 Henv.
+      remember (G1 & X ~ BindTVar k' & G2) as G. gen G2.
+      induction Hkt1; intros; substs; simpls*.
+      { Case "TyFVar". solve_var.
+        + binds_get H0. lets* [Hok ?] : ok_concat_inv (ok_env_ok _ Henv).
+          apply_empty* ok_type_weakening.
+        + binds_cases H0...
+          constructors*. apply binds_concat_right.
+          replaces (BindTVar k) with (bsubst X T2 (BindTVar k))... }
+      { Case "TyAll". assert (Hk : ok_kind (G1 & map (bsubst X T2) G2) k).
+        apply* ok_kind_bsubst. apply* ok_kind_tvar_strengthening.
+        apply_fresh* KAll.
+        assert (lct T2) by apply* ok_type_lct.
+        rewrite~ tsubst_topen_comm.
+        replaces (G1 & map (bsubst X T2) G2 & y ~ BindTVar k)
+          with (G1 & map (bsubst X T2) (G2 & y ~ BindTVar k))...
+        + autorewrite with rew_env_map rew_env_concat ; auto.
+        + apply~ H1.
+          * autorewrite with rew_env_concat ; auto.
+          * autorewrite with rew_env_map rew_env_concat... }
+    Qed.
+
+    Lemma bsubst_ok_env :
+      forall G1 G2 X T2 k,
+        G1 |= T2 ~:: k ->
+        ok_env (G1 & X ~ BindTVar k & G2) ->
+        ok_env (G1 & map (bsubst X T2) G2).
+    Proof.
+      introv Htk Henv.
+      induction G2 using env_ind.
+      { Case "Empty". autorewrite with rew_env_map rew_env_concat in *.
+        apply* ok_env_push. }
+      { Case "Push". autorewrite with rew_env_map rew_env_concat in *.
+        specializes IHG2 (ok_env_push _ _ _ Henv).
+        lets [? Hdisj] : ok_push_inv (ok_env_ok _ Henv).
+        destruct v.
+        { SCase "BindTName". constructor~. }
+        { SCase "BindCon". forwards (Hd & Htk' & HT): ok_env_con_inv Henv.
+          constructor~.
+          - applys ok_data_bsubst. apply* ok_data_tvar_strengthening.
+          - applys* ok_type_tsubst Htk.
+          - binds_cases HT ; auto.
+            replaces BindTName with (bsubst X T2 BindTName) ; auto. }
+        { SCase "BindTVar". forwards Hk: ok_env_tvar_inv Henv.
+          constructor~. applys ok_kind_bsubst. apply* ok_kind_tvar_strengthening. }
+        { SCase "BindVar". forwards Htk': ok_env_var_inv Henv.
+          constructor~. applys* ok_type_tsubst Htk'. }
+        { SCase "BindMatch". constructor~. } }
+    Qed.
+
+    Lemma ok_env_concat :
+      forall G1 G2,
+        ok_env (G1 & G2) ->
+        ok_env G1.
+    Proof with eauto.
+      introv Henv.
+      induction G2 using env_ind.
+      { Case "Empty". rew_env_concat in *... }
+      { Case "Push". apply IHG2. rew_env_concat in *.
+        apply* ok_env_push. }
+    Qed.
+
+    Lemma ok_type_notin :
+      forall Gamma T k X,
+        Gamma |= T ~:: k ->
+        X # Gamma ->
+        X \notin ftv T.
+    Proof.
+      introv Htk Hfresh.
+      induction Htk; simpls*.
+      { Case "TyFVar". intros contra.
+        rewrite in_singleton in contra. substs.
+        apply get_none in Hfresh.
+        apply binds_get in H0.
+        fequals. }
+      { Case "TyAll". pick_fresh Y.
+        forwards~ Hnin: H0 Y.
+        applys~ topen_notin Y. }
+    Qed.
+
+    Lemma env_bsubst_fresh :
+      forall Gamma X T2,
+        ok_env Gamma ->
+        X # Gamma ->
+        Gamma = map (bsubst X T2) Gamma.
+    Proof with eauto using ok_env_push.
+      introv Henv Hfresh.
+      induction Gamma using env_ind.
+      { Case "Empty". rewrite~ map_empty. }
+      { Case "Push". autorewrite with rew_env_map.
+        rewrite <- IHGamma...
+        destruct~ v ; repeat fequals ; unfold bsubst ; rewrite* tsubst_fresh.
+        { SCase "BindCon".
+          apply ok_env_con_inv in Henv as (? & Hkt & ?).
+          apply* ok_type_notin. }
+        { SCase "BindVar".
+          apply ok_env_var_inv in Henv.
+          apply* ok_type_notin. } }
+    Qed.
+
+    Lemma ok_term_tsubst :
+      forall G2 G1 t k T1 T2 X,
+        G1 & X ~ BindTVar k & G2 |= t ~: T1 ->
+        G1 |= T2 ~:: k ->
+        G1 & map (bsubst X T2) G2 |= [{X => T2}]t ~: ({X => T2}T1).
+    Proof with eauto using ok_env_strengthening, bsubst_ok_env with mcore.
+      introv hasType Henv.
+      remember (G1 & X ~ BindTVar k & G2) as G. gen G2.
+      induction hasType; intros; simpls; substs...
+      { Case "TmFVar".
+        binds_cases H0 ; constructors ;
+          replaces (BindVar ({X => T2} ty)) with (bsubst X T2 (BindVar ty))...
+        apply ok_env_concat in H.
+        assert (X # G1) by apply* ok_push_inv.
+        rewrite* (@env_bsubst_fresh G1 X T2). }
+      { Case "TmLam". apply_fresh* TLam as x.
+        + apply* ok_type_tsubst. apply* bsubst_ok_env.
+        + rewrite tsubst_t_open_comm.
+          replaces (G1 & map (bsubst X T2) G2 & x ~ BindVar ({X => T2}ty1))
+            with (G1 & map (bsubst X T2) (G2 & x ~ BindVar ty1)).
+          autorewrite with rew_env_map rew_env_concat ; auto.
+          apply~ H1. rewrite~ concat_assoc. }
+      { Case "TmTyLam". apply_fresh* TTyLam.
+        + apply ok_kind_bsubst. apply* ok_kind_tvar_strengthening.
+        + replaces (G1 & map (bsubst X T2) G2 & y ~ BindTVar k0)
+            with (G1 & map (bsubst X T2) (G2 & y ~ BindTVar k0)).
+          autorewrite with rew_env_map rew_env_concat ; auto.
+          rewrite~ tsubst_topen_comm...
+          rewrite topen_t_tsubst_comm...
+          apply~ H1. rewrite~ concat_assoc. }
+      { Case "TmTyApp".
+        rewrite tsubst_topen_distr... constructors*.
+        apply* ok_type_tsubst. }
+    Qed.
 
   End Typing.
 End Typing.
